theories/Dijkstra/StateIOTrace.v
@@ -24,11 +24,11 @@ From ITree Require Import
      Events.StateFacts
      Core.Divergence
      Dijkstra.DijkstraMonad
-     Dijkstra.ITrace
-     Dijkstra.ITraceBind
-     Dijkstra.EuttDiv
-     Dijkstra.ITracePreds
-     Dijkstra.ITraceBindTrigger
+     ITrace.ITraceDefinition
+     ITrace.ITraceFacts
+     ITrace.ITraceBind
+     ITrace.EuttDiv
+     ITrace.ITracePreds
      Dijkstra.TracesIT
      Dijkstra.StateSpecT
    (*  Simple *)
