theories/ITrace/ITraceDefinition.v
@@ -1,0 +1,111 @@
+From Coq Require Import
+     Arith.PeanoNat
+     Lists.List
+     Strings.String
+     Morphisms
+     Setoid
+     RelationClasses
+     Logic.Classical_Prop
+     Logic.EqdepFacts
+     Program.Equality
+     (* Logic.IndefiniteDescription *)
+.
+
+From ExtLib Require Import
+     Data.String
+     Structures.Monad
+     Structures.Traversable
+     Data.List.
+
+From ITree Require Import
+     ITree
+     ITreeFacts
+     ITrace.EuttEv
+     Divergence
+.
+
+
+From Paco Require Import paco.
+
+Import Monads.
+Import MonadNotation.
+Local Open Scope monad_scope.
+
+Variant EvAns (E : Type -> Type) : Type -> Type :=
+  | evans : forall {A : Type} (ev : E A) (ans : A), EvAns E unit
+  (*if you can prove there is no answers, don't need to proved one*)
+  | evempty : forall {A : Type} (Hempty : A -> void) (ev : E A), EvAns E void
+.
+
+Arguments evans {E}.
+Arguments evempty {E}.
+
+Definition itrace (E : Type -> Type) (R : Type) := itree (EvAns E) R.
+
+Definition itrace' (E : Type -> Type) (R : Type) := itree' (EvAns E) R.
+
+Definition ev_stream (E : Type -> Type) := itrace E unit.
+
+Definition Nil {E : Type -> Type} : ev_stream E := Ret tt.
+
+Definition ev_list (E : Type -> Type) := list (EvAns E unit).
+
+Fixpoint ev_list_to_stream {E : Type -> Type} (l : ev_list E) : ev_stream E :=
+  match l with
+  | nil => Ret tt
+  | e :: t => Vis e (fun _ => ev_list_to_stream t) end.
+
+(*one append for traces and streams, get associativity for free from bind_bind*)
+Definition append {E R} (s : itrace E unit) (b : itrace E R) :=
+  ITree.bind s (fun _ => b).
+
+Notation "s ++ b" := (append s b).
+
+Variant REvRef (E : Type -> Type) : forall (A B : Type), EvAns E A -> E B -> Prop := 
+  | rer {A : Type} (e : E A) (a : A) : REvRef E unit A (evans A e a) e
+  | ree {A : Type} (e : E A) (Hempty : A -> void) : REvRef E void A (evempty A Hempty e) e
+.
+Hint Constructors REvRef.
+
+(*shouldn't need an empty case*)
+Variant RAnsRef (E : Type -> Type) : forall (A B : Type), EvAns E A -> A -> E B -> B -> Prop :=
+  | rar {A : Type} (e : E A) (a : A) : RAnsRef E unit A (evans A e a) tt e a.
+Hint Constructors RAnsRef.
+
+Definition trace_refine {E R}  (t : itree E R) (b : itrace E R)  := 
+   euttEv (REvRef E) (RAnsRef E) eq b t.
+
+
+Notation "b ⊑ t" := (trace_refine t b) (at level 70).
+
+Variant must_divergeF {E : Type -> Type} {A : Type} (F : itree E A -> Prop) : itree' E A -> Prop :=
+  | MDivTau (t : itree E A) : F t -> must_divergeF F (TauF t)
+  | MDivVis (B : Type) (k : B -> itree E A) (e : E B) : 
+      (forall b, F (k b)) -> must_divergeF F (VisF e k).
+Hint Constructors must_divergeF.
+
+Definition must_diverge_ {E A} (sim : itree E A -> Prop) t := must_divergeF sim (observe t).
+
+Lemma must_divergeF_mono {E A} (sim sim' : itree E A -> Prop) t
+      (IN : must_divergeF sim t)
+      (LE : sim <1= sim') : must_divergeF sim' t.
+Proof.
+  induction IN; eauto. 
+Qed.
+
+Lemma must_divergeF_mono' {E A} : monotone1 (@must_diverge_ E A).
+Proof.
+  unfold must_diverge_.
+  red. intros. eapply must_divergeF_mono; eauto.
+Qed.
+Hint Resolve must_divergeF_mono' : paco. 
+
+Definition must_diverge {E A} := paco1 (@must_diverge_ E A) bot1.
+
+Inductive can_converge {E : Type -> Type} {A : Type} (a : A) : itree E A -> Prop :=
+| conv_ret (t : itree E A) : t ≈ Ret a -> can_converge a t
+| conv_vis (t : itree E A ) {B : Type} (e : E B) (k : B -> itree E A) (b : B) : 
+    t ≈ Vis e k -> can_converge a (k b) -> can_converge a t.
+Hint Constructors can_converge.
+
+Definition finite {E : Type -> Type} (s : ev_stream E) : Prop := can_converge tt s.
