theories/ITrace/ITraceFacts.v
@@ -1,0 +1,839 @@
+From Coq Require Import
+     Arith.PeanoNat
+     Lists.List
+     Strings.String
+     Morphisms
+     Setoid
+     RelationClasses
+     Logic.Classical_Prop
+     Logic.EqdepFacts
+     Program.Equality
+     Logic.IndefiniteDescription
+.
+
+From ExtLib Require Import
+     Data.String
+     Structures.Monad
+     Structures.Traversable
+     Data.List.
+
+From ITree Require Import
+     ITree
+     ITreeFacts
+     ITrace.EuttEv
+     Divergence
+     ITrace.ITraceDefinition
+.
+
+
+From Paco Require Import paco.
+
+Import Monads.
+Import MonadNotation.
+Local Open Scope monad_scope.
+
+Lemma classic_empty : forall (A : Type), ( exists e : A + (A -> void), True ).
+Proof.
+  intros. destruct (classic (exists a : A, True)).
+  - destruct H; eauto.
+  - assert (f : A -> void); eauto. intros.
+    exfalso. apply H; eauto.
+Qed.
+
+Global Instance eutt_proper_con_converge {A E} {a : A} : Proper (eutt eq ==> iff) (@can_converge E _ a).
+Proof.
+  intros t1 t2 Ht. split; intros.
+  - induction H.
+    + apply conv_ret; auto. rewrite <- Ht. auto. 
+    + eapply conv_vis with (e0 := e); eauto. rewrite <- H.
+      symmetry. auto.
+  - induction H.
+    + apply conv_ret; auto. rewrite Ht. auto.
+    + eapply conv_vis with (e0 := e); eauto. rewrite Ht.
+      auto.
+Qed.
+
+Ltac contra_void := try match goal with | a : void |- _ => contradiction end. 
+
+Lemma can_converge_trace : forall (E : Type -> Type) (R : Type) 
+                                   (b : itrace E R) (r1 r2 : R),
+    can_converge r1 b -> can_converge r2 b -> r1 = r2.
+Proof.
+  intros. induction H; inversion H0; subst.
+  - rewrite H in H1. pinversion H1. subst. auto.
+  - rewrite H in H1. pinversion H1.
+  - destruct e. destruct b. apply IHcan_converge. rewrite H in H0. inversion H0; subst;
+                                                                    contra_void.
+    + pinversion H3.
+    + destruct e. destruct b. 
+      pinversion H3. apply inj_pair2 in H7. apply inj_pair2 in H8.
+      apply inj_pair2 in H9. apply inj_pair2 in H10. subst.
+      enough (k tt ≈ k0 tt); try apply REL.
+      rewrite H5. auto. contradiction.
+    + contradiction.
+ - destruct e. destruct e0. destruct b. destruct b0.
+   apply IHcan_converge. rewrite H in H2.
+   pinversion H2.
+   repeat match goal with | H : existT _ _ _ = _ |- _ => apply inj_pair2 in H end.
+   subst. enough (k tt ≈ k0 tt); try apply REL.
+   rewrite H4. auto; contra_void.
+   + destruct b0.
+   + destruct b.
+Qed.
+
+Lemma finite_nil {E : Type -> Type} : finite (@Nil E).
+Proof.
+  apply conv_ret. unfold Nil. reflexivity.
+Qed.
+
+Lemma can_converge_list_to_stream : forall (E : Type -> Type) (l : ev_list E),
+    finite (ev_list_to_stream l).
+Proof.
+  red. intros. induction l.
+  - cbn. constructor. reflexivity.
+  - cbn. eapply conv_vis with (e := a) (b := tt); try reflexivity. simpl. auto.
+Qed.
+
+Lemma finite_stream_list : forall (E : Type -> Type) (s : ev_stream E),
+    finite s -> exists l, (s ≈ ev_list_to_stream l)%itree.
+Proof.
+  intros. red in H. induction H.
+  - exists nil. auto.
+  - destruct IHcan_converge as [l Hl]. unfold ev_list in l.
+    inversion e. subst.
+    exists (e:: l). simpl. rewrite H.
+    destruct b. pfold. red. cbn. constructor.
+    intros. destruct v. left. auto.
+    subst. contradiction.
+Qed.
+
+Global Instance eutt_proper_must_diverge {E A R} : Proper (eutt R ==> iff) (@must_diverge E A).
+Proof.
+  intros t1 t2 Ht. split.
+  - revert t1 t2 Ht. pcofix CIH. intros t1 t2 Ht Hdiv.
+    punfold Ht. unfold_eqit. pfold. red. punfold Hdiv. red in Hdiv.
+    induction Ht.
+    + inversion Hdiv.
+    + constructor. inversion Hdiv. subst. right.
+      pclearbot.
+      eapply CIH; eauto.
+    + constructor. inversion Hdiv. subst. apply inj_pair2 in H2.
+      subst. intros. right. inversion Hdiv. subst. apply inj_pair2 in H4.
+      subst. pclearbot. eapply CIH; eauto. apply H2.
+    + apply IHHt. inversion Hdiv. subst. pclearbot. punfold H0.
+    + constructor. left. pfold. apply IHHt. auto.
+  - revert t1 t2 Ht. pcofix CIH. intros t1 t2 Ht Hdiv.
+    punfold Ht. unfold_eqit. pfold. red. punfold Hdiv. red in Hdiv.
+    induction Ht.
+    + inversion Hdiv.
+    + constructor. inversion Hdiv. subst. right.
+      pclearbot.
+      eapply CIH; eauto.
+    + constructor. inversion Hdiv. subst. apply inj_pair2 in H2.
+      subst. intros. right. inversion Hdiv. subst. apply inj_pair2 in H4.
+      subst. pclearbot. eapply CIH; eauto. apply H2.
+    +  constructor. left. pfold. apply IHHt. auto. 
+    +  apply IHHt. inversion Hdiv. subst. pclearbot. punfold H0.
+Qed.
+
+Lemma not_converge_to_must_diverge : forall (E : Type -> Type) (A : Type) (t : itree E A), 
+    (forall a, ~ can_converge a t) -> must_diverge t.
+Proof.
+  intros E A. pcofix CIH. intros t Hcon. pfold.
+  red. destruct (observe t) eqn : Heq;
+         specialize (itree_eta t) as Ht; rewrite Heq in Ht.
+  - exfalso. apply (Hcon r0). rewrite Ht. constructor. reflexivity.
+  - constructor. right. apply CIH.
+    setoid_rewrite Ht in Hcon. setoid_rewrite tau_eutt in Hcon.
+    auto.
+  - constructor. right. apply CIH.
+    intros a Hcontra. setoid_rewrite Ht in Hcon.
+    apply (Hcon a). eapply conv_vis; try reflexivity; eauto.
+Qed.
+
+Lemma classic_converge : forall (E : Type -> Type) (A : Type) (t : itree E A),
+    (exists a, can_converge a t) \/ must_diverge t.
+Proof.
+  intros. destruct (classic (exists a, can_converge a t) ); auto.
+  right. apply not_converge_to_must_diverge. intros a Hcontra.
+  apply H. exists a. auto.
+Qed.
+
+Lemma append_vis : forall (E : Type -> Type) (R : Type)
+                          (e : EvAns E unit) (k : unit -> ev_stream E) (b : itrace E R),
+                          Vis e k ++ b ≈ Vis e (fun a => k a ++ b).
+Proof.
+  intros E R. unfold append. intros.
+  pfold. red. cbn. constructor. intros. left.
+  enough ( (ITree.bind (k v) (fun _ : unit => b) ≈  (ITree.bind (k v) (fun _ : unit => b) ) ) ); auto.
+  reflexivity.
+Qed.
+
+Global Instance proper_append {E R} : Proper (@eutt (EvAns E) unit unit eq ==> @eutt (EvAns E) R R eq ==> eutt eq) (@append E R).
+Proof.
+  intros log1 log2 Hlog b1 b2 Hb. unfold append. rewrite Hlog.
+  eapply eutt_clo_bind; eauto. reflexivity.
+Qed.
+
+Lemma can_converge_append : forall (E : Type -> Type) (R : Type)
+                                   (log : ev_stream E) (r : R),
+      finite log -> can_converge r (log ++ Ret r).
+Proof.
+  intros. induction H.
+  - unfold append. rewrite H. rewrite bind_ret_l.
+    constructor. reflexivity.
+  - rewrite H. inversion e. subst. rewrite append_vis.
+    eapply conv_vis with (e0 := e) (k0 := fun a => k a ++ Ret r); eauto; try reflexivity.
+    subst. contradiction.
+Qed.
+
+Lemma converge_itrace_ev_list : forall (E : Type -> Type) (R : Type) 
+                                        (b : itrace E R) (r : R),
+    can_converge r b -> (exists log, (ev_list_to_stream log) ++ Ret r ≈ b)%itree .
+Proof.
+  intros. induction H.
+  - exists nil. cbn. rewrite H.
+    pfold. red. cbn. constructor. auto.
+  - destruct IHcan_converge as [log Hlog]. inversion e. subst.
+    exists (e :: log). cbn. rewrite append_vis. rewrite H.
+    pfold. red. cbn. constructor. cbn. intros. destruct v.
+    left. destruct b. apply Hlog. subst. contradiction.
+Qed.
+
+Lemma classic_converge_itrace : forall (E : Type -> Type) (R : Type) (b : itrace E R),
+    (exists r, exists log, ( (ev_list_to_stream log) ++ Ret r ≈ b)%itree ) \/ must_diverge b.
+Proof.
+  intros.
+  destruct (classic_converge _ _ b ); auto. destruct H as [r Hr]. left.
+  exists r. apply converge_itrace_ev_list. auto.
+Qed.
+
+Arguments classic_converge_itrace {E} {R}.
+
+Lemma append_nil : forall (E : Type -> Type) (R : Type) (b : itrace E R),
+    (Ret tt ++ b ≈ b)%itree.
+Proof.
+  intros. unfold append. rewrite bind_ret_l. reflexivity.
+Qed.
+
+Lemma append_assoc : forall (E : Type -> Type) (R : Type) (b : itrace E R)
+                            (log log' : ev_list E),
+    ev_list_to_stream (log ++ log')%list ++ b ≈ 
+                      (ev_list_to_stream log) ++ (ev_list_to_stream log') ++ b.
+Proof.
+  intros E R b log. induction log.
+  - simpl. intros. rewrite append_nil. reflexivity.
+  - cbn. intros. rewrite append_vis. setoid_rewrite IHlog.
+    rewrite append_vis. reflexivity.
+Qed.
+
+Lemma append_div : forall (E : Type -> Type) (R : Type) (b : itrace E R)
+                          (log : ev_list E),
+    must_diverge b -> must_diverge ((ev_list_to_stream log) ++ b).
+Proof.
+  intros. induction log.
+  - cbn. unfold append. rewrite bind_ret_l. auto.
+  - cbn. unfold append.
+    pfold. red. cbn. constructor. intros. left. auto.
+Qed.
+
+Lemma inv_append_eutt : forall (E : Type -> Type) (R : Type) (r1 r2 : R)
+                               (log1 log2 : ev_list E),
+    ((ev_list_to_stream log1) ++ Ret r1 ≈ (ev_list_to_stream log2) ++ Ret r2)%itree -> 
+    log1 = log2 /\ r1 = r2.
+Proof.
+  intros. generalize dependent log2. induction log1; intros.
+  - destruct log2.
+    + split; auto. cbn in H. pinversion H. cbn. unfold append in *.
+      cbn in *. subst. auto.
+    + pinversion H.
+  - destruct log2.
+    + pinversion H.
+    + cbn in H. unfold append in H. pinversion H. cbn in *.
+      repeat match goal with H : existT _ _ _ = existT _ _ _ |- _ => apply inj_pair2 in H end.
+      subst.
+      enough (log1 = log2 /\ r1 = r2).
+      { destruct H0. subst. auto. }
+      apply IHlog1. apply REL. apply tt.
+Qed.
+
+Lemma must_diverge_not_converge : forall (E : Type -> Type) (R : Type) (t : itree E R) (r : R),
+    can_converge r t -> ~ must_diverge t.
+Proof.
+  intros E R t r Hc Hd. induction Hc.
+  - rewrite H in Hd. pinversion Hd.
+  - apply IHHc. rewrite H in Hd. pinversion Hd.
+    apply inj_pair2 in H2. apply inj_pair2 in H3. subst.
+    apply H1.
+Qed.
+
+Lemma trace_refine_proper_left' : forall (E : Type -> Type) (R : Type) (b1 b2 : itrace E R)
+                (t : itree E R), (b1 ≈ b2)%itree -> euttEv (REvRef E) (RAnsRef E) eq b1 t -> 
+                                 euttEv (REvRef E) (RAnsRef E) eq b2 t.
+Proof. 
+  intros E R. pcofix CIH. intros. pfold. red.
+  punfold H1. red in H1.  punfold H0. red in H0.
+  genobs_clear t ot3.
+  hinduction H0 before CIH; intros; clear b1 b2; eauto.
+  - remember (RetF r1) as ot1. hinduction H1 before CIH; intros; inv Heqot1; eauto with paco.
+    + constructor. auto.
+    + constructor. eapply IHeuttEvF; eauto.
+  (* Tau Tau case causes the most problems, seems *)
+  -  assert (DEC: (exists m3, ot3 = TauF m3) \/ (forall m3, ot3 <> TauF m3)).
+    { destruct ot3; eauto; right; red; intros; inv H. }
+    destruct DEC as [EQ | EQ].
+    + destruct EQ as [m3 ?]; subst. pclearbot.
+      constructor. right. eapply CIH; eauto.
+      apply euttEv_inv_tauLR. pfold. auto.
+    + inv H1; try (exfalso; eapply EQ; eauto; fail). 
+      pclearbot. constructor.
+      punfold REL. red in REL.
+      hinduction H0 before CIH; intros; subst; try (exfalso; eapply EQ; eauto; fail). 
+      * dependent induction REL; rewrite <- x.
+        ++ constructor. auto.
+        ++ constructor. eapply IHREL; eauto.
+      * eapply IHeuttEvF; eauto. clear IHeuttEvF.
+        dependent induction REL; try (exfalso; eapply EQ; eauto; fail).  
+        ++ pclearbot. rewrite <- x. constructor; auto. pstep_reverse.
+        ++ auto. 
+        ++ rewrite <- x. constructor; auto. eapply IHREL; eauto.
+      * dependent induction REL; rewrite <- x.
+        ++ constructor; auto. intros. apply H0 in H1. right.
+           pclearbot. eapply CIH; eauto.
+        ++ constructor. eapply IHREL; eauto.
+  - remember (VisF e k1) as ot1.
+    hinduction H1 before CIH; intros; dependent destruction Heqot1.
+    + constructor. eapply IHeuttEvF; eauto.
+    + pclearbot. constructor; auto. intros. apply H0 in H1. 
+      pclearbot. right.
+      eapply CIH; eauto.
+  - eapply IHeqitF. remember (TauF t1) as otf1. 
+    hinduction H1 before CIH; intros;  dependent destruction Heqotf1; eauto.
+    + constructor. pclearbot. pstep_reverse.
+    + constructor. eapply IHeuttEvF; eauto.
+  - constructor. eapply IHeqitF. eauto.
+
+Qed. 
+
+Lemma trace_refine_proper_right' : forall (E : Type -> Type) (R : Type) (b : itrace E R)
+                                   (t1 t2 : itree E R), t1 ≈ t2 -> euttEv (REvRef E) (RAnsRef E) eq b t1 -> 
+                                 euttEv (REvRef E) (RAnsRef E) eq b t2.
+Proof.
+  intros E R. pcofix CIH. intros. punfold H1. red in H1.
+  punfold H0. red in H0. pfold. red.
+  genobs_clear t2 ot2.
+  hinduction H0 before CIH; intros; clear t1; subst; eauto.
+  - remember (RetF r2) as ot1. hinduction H1 before CIH; intros; inv Heqot1; eauto with paco.
+    + constructor; auto.
+    + constructor. eauto.
+  - pclearbot. remember (TauF m1) as otm1.
+    hinduction H1 before CIH; intros; subst; try (inv Heqotm1).
+    + constructor. pclearbot. right. eapply CIH; eauto.
+    + constructor. right. eapply CIH; eauto.
+      apply euttEv_inv_tauR. pfold. auto.
+    + punfold REL. red in REL. 
+      dependent induction REL; subst.
+      * constructor. clear IHeuttEvF.
+        hinduction H1 before CIH; intros; dependent destruction x0.
+        ++ rewrite <- x. constructor. auto.
+        ++ constructor. auto.
+      * eapply IHeuttEvF with (m2 := m0); auto.
+        pclearbot. pfold. red. rewrite <- x. constructor; auto.
+        punfold REL.
+      * constructor. rewrite <- x.
+        clear IHeuttEvF. hinduction H1 before CIH; intros; dependent destruction x0.
+        ++ constructor. eapply IHeuttEvF; eauto.
+        ++ constructor; auto. intros. apply H0 in H1.
+           pclearbot. right. eapply CIH; eauto. apply REL.
+      * eapply IHeuttEvF; eauto.
+      * constructor. rewrite <- x. eapply IHREL; eauto.
+  - remember (VisF e k1) as ot1. hinduction H1 before CIH; intros; inv Heqot1.
+    + constructor. eauto.
+    + apply inj_pair2 in H4. apply inj_pair2 in H3. subst.
+      constructor; auto. intros. apply H0 in H1.
+      right. pclearbot. eapply CIH; eauto; apply REL.
+  - eapply IHeqitF; eauto. remember (TauF t0) as otf0.
+    hinduction H1 before CIH; intros; dependent destruction Heqotf0; eauto.
+    + constructor. pclearbot. pstep_reverse.
+    + constructor. eapply IHeuttEvF; eauto.
+  - constructor. eapply IHeqitF. eauto.
+Qed.
+
+Instance trace_refine_proper {E R} : Proper (@eutt E R R eq ==> eutt eq ==> iff) trace_refine.
+Proof.
+  intros b1 b2 Heuttb t1 t2 Heuttt.
+  split; intros;
+  try (eapply trace_refine_proper_right'; [eauto | eapply trace_refine_proper_left'; eauto]);
+  auto; symmetry; auto.
+Qed.
+
+Lemma trace_refine_ret : forall (E : Type -> Type) (R : Type) (r : R),
+    @trace_refine E R (Ret r) (Ret r).
+Proof.
+  intros. pfold. constructor. auto.
+Qed.
+
+Lemma trace_refine_ret_inv_r : forall (E : Type -> Type) (R : Type) (r : R)
+                                     (t : itree E R),
+    Ret r ⊑ t -> t ≈ Ret r.
+Proof.
+  intros. pfold. red. punfold H. red in H. cbn in *.
+  dependent induction H; subst.
+  - rewrite <- x. constructor. auto.
+  - rewrite <- x. constructor; auto.
+Qed.
+
+Lemma trace_refine_ret_inv_l : forall (E : Type -> Type) (R : Type) (r : R)
+                                     (b : itrace E R),
+    b ⊑ Ret r -> (b ≈ Ret r)%itree.
+Proof.
+  intros. pfold. red. punfold H. red in H. cbn in *.
+  dependent induction H; subst.
+  - rewrite <- x. constructor. auto.
+  - rewrite <- x. constructor; auto.
+Qed.
+
+Lemma trace_refine_vis_inv : forall (E : Type -> Type) (R A: Type) (e : E A) (a : A)
+                                     (b :itrace E R) (k : A -> itree E R),
+    trace_refine (Vis e k) (Vis (evans A e a) (fun _ => b))  -> trace_refine (k a) b .
+Proof.
+  intros E R A e a. intros.
+  red in H. red. punfold H. red in H. inversion H. 
+  repeat match goal with H : existT _ _ _ = _ |- _ => apply inj_pair2 in H end.
+  subst. 
+  assert (RAnsRef E unit A (evans A e a) tt e a); eauto.
+  apply H7 in H0. pclearbot. auto.
+Qed.
+
+Lemma trace_refine_vis_add : forall (E : Type -> Type) (R A: Type) (e : E A) (a : A)
+                                     (b :itrace E R) (k : A -> itree E R),
+    b ⊑ k a -> Vis (evans A e a) (fun _ => b) ⊑ Vis e k.
+Proof.
+  intros. pfold. red. cbn. constructor; eauto.
+  intros. left. inversion H0.
+  repeat match goal with H : existT _ _ _ = _   |- _ => apply inj_pair2 in H end.
+  subst. auto.
+Qed.
+
+Lemma event_ans_constr : forall (E : Type -> Type) (R : Type) (e : E R),
+    exists (A : Type), exists e' : EvAns E A, REvRef E A R e' e.
+Proof.
+  intros.
+  destruct (classic_empty R) as  [ [a | Hempty]  _ ] .
+  - exists unit. exists (evans R e a). eauto.
+  - exists void. exists (evempty R Hempty e). eauto.
+Qed.
+
+(* Here are where some of the sketchy uses of axioms are *)
+
+CoFixpoint determinize_ (E : Type -> Type) (R : Type) (ot : itree' E R) : itrace E R.
+  destruct ot.
+- apply (Ret r).
+- apply (Tau (determinize_ E R (observe t) ) ).
+- specialize (classic_empty X) as H. 
+  apply constructive_indefinite_description in H. destruct H as [ [x | f] _].
+  + apply (Vis (evans X e x) (fun _ =>  (determinize_ E R (observe (k x)) ) )) .
+  + apply (Vis (evempty X f e) (fun v : void => match v return itrace E R with end)  ).
+Defined.
+
+Definition determinize {E R} t := determinize_ E R (observe t).
+
+(* may be a better idea to make this an axiom *)
+Lemma itree_refine_nonempty : forall (E : Type -> Type) (R : Type) (t : itree E R),
+    exists b : itrace E R, b ⊑ t.
+Proof.
+  intros. exists (determinize t). generalize dependent t.
+  pcofix CIH. intros. pfold. red. unfold determinize. destruct (observe t).
+  - cbn. constructor. auto.
+  - cbn. constructor. right. apply CIH.
+  - unfold observe. cbn. cbn. destruct (constructive_indefinite_description (fun _ : X + (X -> void) => True)
+                   (classic_empty X)).
+    destruct x as [x | f]; cbn.
+    + constructor; eauto. intros. right. 
+      inversion H. 
+      repeat match goal with | H : existT _ _ _ = _ |- _ => apply inj_pair2 in H end.
+      subst. apply CIH.
+    + constructor; auto. intros. contradiction. 
+Qed.
+
+
+Lemma refine_set_eq_to_eutt_vis_aux : forall (E : Type -> Type) (R : Type) (r : itree E R -> itree E R -> Prop)
+      (CIH : forall t1 t2 : itree E R, (forall b : itrace E R, b ⊑ t1 <-> b ⊑ t2) -> r t1 t2)
+      (t1 t2 : itree E R)
+      (H0 : forall b : itrace E R, b ⊑ t1 <-> b ⊑ t2)
+      (A B : Type) (e : E A) (e0 : E B)
+      (k : A -> itree E R) (k0 : B -> itree E R)
+      (Ht1 : t1 ≅ Vis e k) (Ht2 : t2 ≅ Vis e0 k0 ),
+      eqitF eq true true id (upaco2 (eqit_ eq true true id) r) (VisF e k) (VisF e0 k0).
+Proof.
+  intros.
+  destruct (classic_empty A) as [ [a | Ha] _ ].
+  - specialize  trace_refine_vis_add with (e := e) (k := k) (a := a) as Hbrv.
+    assert (exists b, b ⊑ (k a) ). 
+    { apply itree_refine_nonempty. }
+    destruct H as [b Hbk]. apply trace_refine_vis_add with (e := e) in Hbk.
+    rewrite <- Ht1 in Hbk.
+    apply H0 in Hbk as Hbk0.
+    rewrite Ht1 in Hbk. rewrite Ht2 in Hbk0.
+    pinversion Hbk.
+    pinversion Hbk0.
+    repeat match goal with | H : existT _ _ _ = _ |- _ => apply inj_pair2 in H end.
+    subst.
+    inversion H10.
+    repeat match goal with | H : existT _ _ _ = _ |- _ => apply inj_pair2 in H end.
+    subst.
+    repeat match goal with | H : existT _ _ _ = _ |- _ => apply inj_pair2 in H end.
+    subst. constructor.
+    intros. right. eapply CIH; eauto.
+    intros. setoid_rewrite Ht1 in H0. setoid_rewrite Ht2 in H0.
+    split; intros.
+    + apply trace_refine_vis_add with (e := e) in H. apply H0 in H.
+      apply trace_refine_vis_inv in H. auto.
+    + apply trace_refine_vis_add with (e := e) in H. apply H0 in H.
+      apply trace_refine_vis_inv in H. auto.
+  - set (fun v : void => match v return itrace E R with end) as ke.
+    set (Vis (evempty A Ha e) ke) as b.
+    assert (b ⊑ t1).
+    {
+      unfold b. rewrite Ht1. pfold. red. cbn.
+      constructor; intuition.
+    }
+    apply H0 in H as H1. unfold b in *. clear b.
+    rewrite Ht1 in H. rewrite Ht2 in H1.
+    pinversion H. pinversion H1.
+    repeat match goal with | H : existT _ _ _ = _ |- _ => apply inj_pair2 in H end.
+    subst. inversion H12.
+    repeat match goal with | H : existT _ _ _ = _ |- _ => apply inj_pair2 in H end.
+    subst.
+    repeat match goal with | H : existT _ _ _ = _ |- _ => apply inj_pair2 in H end.
+    subst.
+    constructor.
+    intros. right. eapply CIH.
+    intros. setoid_rewrite Ht1 in H0. setoid_rewrite Ht2 in H0.
+    split; intros; contradiction.
+Qed.
+
+Lemma trace_refine_vis : forall (E : Type -> Type) (R A : Type) (b : itrace E R)
+                                 (e : E A) (k : A -> itree E R),
+    b ⊑ Vis e k -> exists X, exists e0 : EvAns E X, exists k0, (b ≈ Vis e0 k0)%itree.
+Proof.
+  intros. punfold H. red in H. cbn in H.
+  dependent induction H.
+  - enough 
+      (exists (X : Type) (e0 : EvAns E X) (k0 : X -> itree (EvAns E) R), (t1 ≈ Vis e0 k0)%itree).
+    {
+      destruct H0 as [ X [e0 [k0 Ht1] ] ].
+      exists X. exists e0. exists k0.
+      specialize (itree_eta b) as Hb. rewrite <- x in Hb. rewrite Hb.
+      rewrite tau_eutt. auto.
+    }
+    eapply IHeuttEvF; eauto.
+  - exists A0. exists e1. exists k1.
+    specialize (itree_eta b) as Hb. rewrite <- x in Hb.
+    rewrite Hb. reflexivity.
+Qed.
+
+Ltac inj_existT := repeat match goal with | H : existT _ _ _ = _ |- _ => apply inj_pair2 in H end.
+
+
+Lemma trace_refine_vis_l : forall (E : Type -> Type) (R A: Type) (t : itree E R)
+                                   (e : EvAns E A) (k : A -> itrace E R),
+    Vis e k ⊑ t -> exists X, exists e0 : E X, exists k0 : X -> itree E R, t ≈ Vis e0 k0.
+Proof.
+  intros. punfold H. red in H. cbn in *.
+  dependent induction H.
+  - assert (t2 ≈ t).
+    {
+      specialize (itree_eta t). rewrite <- x. intros.
+      rewrite H0. rewrite tau_eutt. reflexivity.
+    }
+    setoid_rewrite <- H0. eapply IHeuttEvF; eauto.
+  - exists B. exists e2.  exists k2. specialize (itree_eta t) as Ht.
+      rewrite <- x in Ht. rewrite Ht. reflexivity.
+Qed.
+
+Lemma trace_refine_can_converge_ex : forall (E : Type -> Type) (R : Type)
+                         (t : itree E R) (r : R),
+    can_converge r t -> exists b, can_converge r b /\ b ⊑ t.
+Proof.
+  intros. induction H.
+  - exists (Ret r). rewrite H. split.
+    + constructor. reflexivity.
+    + apply trace_refine_ret.
+  - destruct IHcan_converge as [br [Hrbr Hrefbr] ].
+    exists  (Vis (evans B e b) (fun _ => br) ). split.
+    + eapply conv_vis with (b0 := tt); try reflexivity. auto.
+    + rewrite H. apply trace_refine_vis_add. auto.
+Qed.
+
+Lemma trace_refine_can_converge : forall (E : Type -> Type) (R : Type)
+                         (t : itree E R) (r : R) (b : itrace E R),
+    can_converge r b -> b ⊑ t -> can_converge r t.
+Proof.
+  intros. generalize dependent t. induction H; intros.
+  - rewrite H in H0. apply trace_refine_ret_inv_r in H0.
+    rewrite H0. constructor. reflexivity.
+  - rewrite H in H1. apply trace_refine_vis_l in H1 as Ht0.
+    destruct Ht0 as [X [e0 [k0 Ht0] ] ].
+    rewrite Ht0 in H1. pinversion H1. subst.
+    inj_existT. subst. rewrite Ht0. 
+    inversion H4; subst; inj_existT; subst; try contradiction.
+    eapply conv_vis with (b0 := a); try reflexivity.
+    apply IHcan_converge. pclearbot.
+    specialize (H9 tt a). assert (RAnsRef E unit X (evans X e0 a) tt e0 a).
+    constructor. apply H9 in H2. pclearbot. destruct b. auto.
+Qed.
+
+Lemma trace_refine_must_diverge : forall (E : Type -> Type) (R : Type)
+                       (t : itree E R) (b : itrace E R),
+    must_diverge t -> b ⊑ t -> must_diverge b.
+Proof.
+  intros E R. pcofix CIH. intros. punfold H0. red in H0.
+  punfold H1. red in H1. pfold. red. dependent induction H1.
+  - rewrite <- x in H0. inversion H0.
+  - rewrite <- x0. constructor. right. pclearbot. eapply CIH; eauto.
+    rewrite <- x in H0. inv H0. pclearbot. auto.
+  - rewrite <- x. constructor. left.  pfold. eapply IHeuttEvF; eauto.
+  - eapply IHeuttEvF; auto. rewrite <- x in H0. inv H0.
+    pclearbot. punfold H2.
+  - rewrite <- x0. rewrite <- x in H0. constructor. inv H0.
+    inj_existT. subst. intros. right. pclearbot. 
+    inversion H; subst; inj_existT; subst; try contradiction. destruct b0. clear H5.
+    eapply CIH; try apply H3.
+    specialize (H1 tt a). assert (RAnsRef _ _ _ (evans B e2 a) tt e2 a ).
+    constructor. apply H1 in H0. unfold id in H0.
+    destruct H0; try contradiction. eauto.
+Qed.
+
+Lemma trace_refine_converge_bind : forall (E : Type -> Type) (R S : Type)
+            (b : itrace E R) (t : itree E R) (f : R -> itrace E S) (g : R -> itree E S) (r : R),
+    can_converge r b -> b ⊑ t -> f r ⊑ g r -> ITree.bind b f ⊑ ITree.bind t g.
+Proof.
+  intros. generalize dependent t. dependent induction H; intros.
+  - rewrite H. rewrite H in H0. apply trace_refine_ret_inv_r in H0. 
+    rewrite H0. repeat rewrite bind_ret_l. auto.
+  - specialize (IHcan_converge H1). 
+    rewrite H in H2. apply trace_refine_vis_l in H2 as Ht.
+    destruct Ht as [X [e0 [k0 Ht] ] ].
+    rewrite Ht in H2. punfold H2. red in H2. cbn in H2. inversion H2; subst.
+    inj_existT. subst. pclearbot.
+    inversion H5; inj_existT; subst; try contradiction.
+    inj_existT. subst. rewrite H. rewrite Ht.
+    pfold. red. cbn. constructor; auto.
+    intros. apply H10 in H3. pclearbot. left. 
+    destruct a0. destruct b. apply IHcan_converge. auto.
+Qed.
+
+Lemma trace_refine_diverge_bind : forall (E : Type -> Type) (R S : Type)
+                  (b : itrace E R) (t : itree E R) (f : R -> itrace E S) (g : R -> itree E S),
+    must_diverge b -> b ⊑ t -> ITree.bind b f ⊑ ITree.bind t g.
+Proof.
+  intros E R S b t f g. generalize dependent b. generalize dependent t.
+  pcofix CIH. intros.
+  punfold H0. red in H0.
+  punfold H1. red in H1. pfold. red. cbn. 
+  dependent induction H1.
+  - rewrite <- x0 in H0. inv H0.
+  - unfold observe. cbn. rewrite <- x0. rewrite <- x.
+    cbn. constructor. right. pclearbot. apply CIH; auto.
+    rewrite <- x0 in H0. inv H0. pclearbot. auto.
+  - unfold observe at 1. cbn. rewrite <- x. cbn. constructor.
+    eapply IHeuttEvF; eauto. rewrite <- x in H0. inv H0. pclearbot. pstep_reverse.
+  - unfold observe at 2. cbn. rewrite <- x. cbn. constructor. 
+    eapply IHeuttEvF; eauto.
+  - unfold observe. cbn. rewrite <- x0. rewrite <- x. cbn. constructor; auto.
+    intros.
+    rewrite <- x0 in H0. inv H0. inj_existT. subst. pclearbot.
+    apply H1 in H2. right. eapply CIH; eauto; try apply H4.
+    unfold id in H2. pclearbot. auto.
+Qed.
+
+Lemma refine_set_eq_to_eutt : forall (E : Type -> Type) (R : Type) (t1 t2 : itree E R),
+    (forall b, b ⊑ t1 <-> b ⊑ t2) -> t1 ≈ t2.
+Proof.
+  intros E R. pcofix CIH. intros.
+  pfold. red.
+  remember (observe t1) as ot1. remember (observe t2) as ot2.
+  destruct (ot1); destruct (ot2).
+    (*Ret Ret*)
+  - specialize (H0 (Ret r0) ) as Hr0.
+    specialize (itree_eta t1) as Ht1. rewrite <- Heqot1 in Ht1.
+    specialize (itree_eta t2) as Ht2. rewrite <- Heqot2 in Ht2.
+    rewrite Ht1 in Hr0. rewrite Ht2 in Hr0.
+    assert (Ret r0 ⊑ t2).
+    { rewrite Ht2. apply Hr0. pfold. constructor. auto. }
+    rewrite Ht2 in H. pinversion H. subst. constructor. auto.
+    (*Ret Tau *)
+  - specialize (itree_eta t1) as Ht1. rewrite <- Heqot1 in Ht1.
+    specialize (itree_eta t2) as Ht2. rewrite <- Heqot2 in Ht2.
+    setoid_rewrite Ht2 in H0.
+    specialize (H0 (Ret r0) ).
+    rewrite tau_eutt in H0. constructor; auto.
+    assert (Ret r0 ⊑ t1).
+    { rewrite Ht1. pfold. constructor. auto. }
+    apply H0 in H. punfold H. red in H. cbn in H.
+    clear H0 Ht1 Ht2 Heqot1 Heqot2. dependent induction H.
+    + rewrite <- x. constructor; auto.
+    + rewrite <- x. constructor; auto.
+    (*Ret Vis*)
+  - exfalso.
+    specialize (itree_eta t1) as Ht1. rewrite <- Heqot1 in Ht1.
+    specialize (itree_eta t2) as Ht2. rewrite <- Heqot2 in Ht2.
+    assert (Ret r0 ⊑ t1).
+    { rewrite Ht1. pfold. constructor. auto. }
+    apply H0 in H. rewrite Ht2 in H. pinversion H.
+    (*Tau Ret*)
+  - specialize (itree_eta t1) as Ht1. rewrite <- Heqot1 in Ht1.
+    specialize (itree_eta t2) as Ht2. rewrite <- Heqot2 in Ht2.
+    setoid_rewrite Ht1 in H0. setoid_rewrite Ht2 in H0.
+    assert (Ret r0 ⊑ t2).
+    { rewrite Ht2. pfold. constructor. auto. }
+     rewrite Ht2 in H. apply H0 in H as H1. punfold H1.
+    clear Heqot1 Heqot2 Ht1 Ht2 H H0. red in H1. cbn in *.
+    constructor; auto. inv H1. dependent induction H2; intros; subst.
+    + rewrite <- x. auto.
+    + rewrite <- x. constructor; auto.
+    (*Tau Tau*)
+  - constructor. right. eapply CIH. 
+    intros. 
+    specialize (itree_eta t1) as Ht1. rewrite <- Heqot1 in Ht1.
+    specialize (itree_eta t2) as Ht2. rewrite <- Heqot2 in Ht2.
+    assert (t1 ≈ t). { rewrite Ht1. rewrite tau_eutt. reflexivity. }
+    assert (t2 ≈ t0). { rewrite Ht2. rewrite tau_eutt. reflexivity. }
+    rewrite <- H. rewrite <- H1. auto.
+    (*Tau Vis*)
+  - specialize (itree_eta t1) as Ht1. rewrite <- Heqot1 in Ht1.
+    specialize (itree_eta t2) as Ht2. rewrite <- Heqot2 in Ht2. 
+    specialize (itree_refine_nonempty _ _ (t1) ) as [b Hbt1].
+    apply H0 in Hbt1 as Hbt2. rewrite Ht1 in Hbt1.
+    rewrite tau_eutt in Hbt1. 
+    rewrite Ht2 in Hbt2.
+    apply trace_refine_vis in Hbt2 as Hb.
+    destruct Hb as [Y [e0 [k0 Hb] ] ].
+    rewrite Hb in Hbt2.
+    rewrite Hb in Hbt1. clear Hb b.
+    constructor; auto. 
+    setoid_rewrite Ht1 in H0. setoid_rewrite tau_eutt in H0.
+    clear Heqot1 Heqot2. clear Ht1 t1.
+    punfold Hbt1. red in Hbt1. cbn in *.
+    dependent induction Hbt1.
+    + rewrite <- x. constructor; auto. eapply IHHbt1; eauto.
+      assert (t0 ≈ t).
+      { 
+        specialize (itree_eta t) as Ht. rewrite <- x in Ht. rewrite Ht.
+        rewrite tau_eutt. reflexivity. 
+      }
+      setoid_rewrite H. auto.
+    + rewrite <- x.
+      specialize (itree_eta t) as Ht. rewrite <- x in Ht.
+      eapply refine_set_eq_to_eutt_vis_aux; eauto.
+    (*Vis Ret*)
+  - exfalso.
+    specialize (itree_eta t1) as Ht1. rewrite <- Heqot1 in Ht1.
+    specialize (itree_eta t2) as Ht2. rewrite <- Heqot2 in Ht2.
+    assert (Ret r0 ⊑ t2).
+    { rewrite Ht2. pfold. constructor. auto. }
+    apply H0 in H. rewrite Ht1 in H. pinversion H.
+    (*Vis Tau*)
+  - specialize (itree_eta t1) as Ht1. rewrite <- Heqot1 in Ht1.
+    specialize (itree_eta t2) as Ht2. rewrite <- Heqot2 in Ht2. 
+    specialize (itree_refine_nonempty _ _ (t2) ) as [b Hbt2].
+    apply H0 in Hbt2 as Hbt1. rewrite Ht1 in Hbt1.
+    rewrite Ht2 in Hbt2.
+    rewrite tau_eutt in Hbt2. 
+    apply trace_refine_vis in Hbt1 as Hb.
+    destruct Hb as [Y [e0 [k0 Hb] ] ].
+    rewrite Hb in Hbt2.
+    rewrite Hb in Hbt1. clear Hb b.
+    constructor; auto. 
+    setoid_rewrite Ht2 in H0. setoid_rewrite tau_eutt in H0.
+    clear Heqot1 Heqot2. clear Ht2 t2.
+    punfold Hbt2. red in Hbt2. cbn in *.
+    dependent induction Hbt2.
+    + rewrite <- x. constructor; auto. eapply IHHbt2; eauto.
+      assert (t2 ≈ t).
+      { 
+        specialize (itree_eta t) as Ht. rewrite <- x in Ht. rewrite Ht.
+        rewrite tau_eutt. reflexivity. 
+      }
+      setoid_rewrite H. auto.
+    + rewrite <- x.
+      specialize (itree_eta t) as Ht. rewrite <- x in Ht.
+      eapply refine_set_eq_to_eutt_vis_aux; eauto.
+    (*Vis Vis*)
+  - specialize (itree_eta t1) as Ht1. rewrite <- Heqot1 in Ht1.
+    specialize (itree_eta t2) as Ht2. rewrite <- Heqot2 in Ht2.
+    eapply refine_set_eq_to_eutt_vis_aux; eauto.
+Qed.
+
+Lemma trace_set_complete : forall E R (t1 t2 : itree E R), (forall b, b ⊑ t1 <-> b ⊑ t2) <-> t1 ≈ t2.
+Proof.
+  intros. split; intros; try apply refine_set_eq_to_eutt; auto.
+  rewrite H. split; auto.
+Qed.
+
+
+Lemma paco2_eqit_refl : forall E R r (t : itree E R), paco2 (eqit_ eq true true id) r t t.
+Proof.
+  intros. eapply paco2_mon with (r := bot2); intuition.
+  enough (t ≈ t); auto. reflexivity.
+Qed.
+
+Lemma trace_refine_bind_cont_inv : forall (E : Type -> Type) (R S : Type)
+         (b : itrace E R) (m : itree E R) (g : R -> itrace E S)
+         (f : R -> itree E S) (r : R),
+    can_converge r b -> b ⊑ m -> ITree.bind b g ⊑ ITree.bind m f -> g r ⊑ f r.
+Proof.
+  intros E R S. pcofix CIH. intros b m g f a Hconv Hrefb Hrefbind.
+  generalize  dependent m.
+  dependent induction  Hconv; intros m Hrefb Hrefbind.
+  - rewrite H in Hrefbind. rewrite bind_ret_l in Hrefbind. rewrite H in Hrefb.
+    apply trace_refine_ret_inv_r in Hrefb. rewrite Hrefb in Hrefbind.
+    rewrite bind_ret_l in Hrefbind. eapply paco2_mon; eauto. intuition.
+  - (*m must be a vis, the continuations must refine then continuation in the m I use in the 
+      inductive hypothesis *)
+    destruct e; try contradiction. rewrite H in Hrefb.
+    rewrite H in Hrefbind. rewrite bind_vis in Hrefbind.
+    apply trace_refine_vis_l in Hrefb as Hvis. destruct Hvis as [X [e' [k' Hvis ] ] ].
+    rewrite Hvis in Hrefbind. rewrite bind_vis in Hrefbind.
+    punfold Hrefbind. red in Hrefbind. cbn in Hrefbind. inv Hrefbind.
+    inj_existT; subst. inv H2. inj_existT; subst.
+    rewrite Hvis in Hrefb. punfold Hrefb. red in Hrefb. cbn in Hrefb. inv Hrefb.
+    inj_existT; subst.
+    assert (RAnsRef E unit A (evans _ ev ans) tt ev ans ); try (constructor; auto; fail).
+    specialize (IHHconv (k' ans) ). apply IHHconv.
+    + apply H8 in H0. pclearbot. destruct b. auto.
+    + apply H7 in H0. pclearbot. destruct b. auto.
+Qed.
+
+Lemma can_converge_two_list:
+  forall (E : Type -> Type) (A B : Type) (log : ev_list E) (b : itrace E A) 
+    (a : A) (log' : ev_list E),
+    (ev_list_to_stream log) ++ b ≈ (ev_list_to_stream log') ++ Ret a -> can_converge a b.
+Proof.
+  intros. generalize dependent log'.
+  induction log; cbn; intros.
+  - simpl in H. setoid_rewrite bind_ret_l in H. rewrite H.
+    apply can_converge_append. apply can_converge_list_to_stream.
+  - assert ((Vis a0 (fun _ => ev_list_to_stream log)) ≈ ev_list_to_stream (a0 :: log) )%itree.
+    { cbn. reflexivity. }
+    rewrite H0 in H.
+    destruct log' as [ | h t ].
+    + setoid_rewrite bind_ret_l in H. simpl in H. pinversion H.
+    + simpl in H. unfold append in H. repeat rewrite bind_vis in H. pinversion H.
+      inj_existT; subst.
+      assert (ev_list_to_stream log ++ b ≈ ev_list_to_stream t ++ Ret a).
+      { apply REL. apply tt. }
+      eapply IHlog; eauto.
+Qed.
+
+Lemma must_diverge_bind_append: forall (E : Type -> Type) (A : Type) 
+                                  (log : ev_list E) (b' : itree (EvAns E) A),
+    must_diverge (ev_list_to_stream log ++ b') -> must_diverge b'.
+Proof.
+  intros E A log b' Hdiv. induction log.
+  - cbn in Hdiv. setoid_rewrite bind_ret_l in Hdiv. auto.
+  - apply IHlog. simpl in Hdiv. unfold append in Hdiv.
+    rewrite bind_vis in Hdiv. pinversion Hdiv. inj_existT. subst. apply H0.
+    apply tt.
+Qed.
